Allow users to specify the tag of the events

src/lib/communication/DY.Lib.Communication.Core.fst
@@ -19,9 +19,6 @@ let comm_layer_pkenc_tag = "DY.Lib.Communication.PkEnc.PublicKey"
 val comm_layer_sign_tag: string
 let comm_layer_sign_tag = "DY.Lib.Communication.Sign.PublicKey"
 
-val comm_layer_event_tag: string
-let comm_layer_event_tag = "DY.Lib.Communication.Event.Core"
-
 type communication_keys_sess_ids = {
   pki: state_id;
   private_keys: state_id;
@@ -48,8 +45,12 @@ type communication_event =
 %splice [ps_communication_event_is_well_formed] (gen_is_well_formed_lemma (`communication_event))
 #pop-options
 
-instance event_communication_event: event communication_event = {
-  tag = comm_layer_event_tag;
+class comm_layer_event_core_tag = {
+  tag: string;
+}
+
+instance event_communication_event {|t:comm_layer_event_core_tag|}: event communication_event = {
+  tag = t.tag;
   format = mk_parseable_serializeable ps_communication_event;
 }
 
@@ -67,11 +68,12 @@ let encrypt_message #a pk_receiver nonce payload =
 
 [@@ "opaque_to_smt"]
 val send_confidential:
-  #a:Type -> {| parseable_serializeable bytes a |} ->
+  {|comm_layer_event_core_tag|} ->
+  #a:Type0 -> {| parseable_serializeable bytes a |} ->
   communication_keys_sess_ids ->
   principal -> principal -> a ->
   traceful (option timestamp)
-let send_confidential #a comm_keys_ids sender receiver payload =
+let send_confidential #event_tag #a comm_keys_ids sender receiver payload =
   let*? pk_receiver = get_public_key sender comm_keys_ids.pki (LongTermPkeKey comm_layer_pkenc_tag) receiver in
   let* nonce = mk_rand PkeNonce (long_term_key_label sender) 32 in
   trigger_event sender (CommConfSendMsg sender receiver (serialize a payload));*
@@ -89,11 +91,12 @@ let decrypt_message #a sk_receiver msg_encrypted =
 
 [@@ "opaque_to_smt"]
 val receive_confidential:
+  {|comm_layer_event_core_tag|} ->
   #a:Type -> {| parseable_serializeable bytes a |} ->
   communication_keys_sess_ids ->
   principal -> timestamp ->
   traceful (option a)
-let receive_confidential #a comm_keys_ids receiver msg_id =
+let receive_confidential #event_tag #a comm_keys_ids receiver msg_id =
   let*? sk_receiver = get_private_key receiver comm_keys_ids.private_keys (LongTermPkeKey comm_layer_pkenc_tag) in
   let*? msg_encrypted = recv_msg msg_id in
   let*? payload = return (decrypt_message #a sk_receiver msg_encrypted) in
@@ -123,11 +126,12 @@ let sign_message #a sender receiver payload pk_receiver sk nonce =
 
 [@@ "opaque_to_smt"]
 val send_authenticated:
+  {|comm_layer_event_core_tag|} ->
   #a:Type -> {| parseable_serializeable bytes a |} ->
   communication_keys_sess_ids ->
   principal -> principal -> a ->
   traceful (option timestamp)
-let send_authenticated #a comm_keys_ids sender receiver payload =
+let send_authenticated #event_tag #a comm_keys_ids sender receiver payload =
   let*? sk_sender = get_private_key sender comm_keys_ids.private_keys (LongTermSigKey comm_layer_sign_tag) in
   let* nonce = mk_rand SigNonce (long_term_key_label sender) 32 in
   let payload_bytes = serialize a payload in
@@ -174,11 +178,12 @@ let get_sender sign_msg_bytes =
 
 [@@ "opaque_to_smt"]
 val receive_authenticated:
+  {|comm_layer_event_core_tag|} ->
   #a:Type -> {| parseable_serializeable bytes a |} ->
   communication_keys_sess_ids ->
   principal -> timestamp ->
   traceful (option (communication_message a))
-let receive_authenticated #a comm_keys_ids receiver msg_id =
+let receive_authenticated #event_tag #a comm_keys_ids receiver msg_id =
   let*? msg_signed_bytes = recv_msg msg_id in
   let*? sender = return (get_sender msg_signed_bytes) in
   let*? vk_sender = get_public_key receiver comm_keys_ids.pki (LongTermSigKey comm_layer_sign_tag) sender in
@@ -203,11 +208,12 @@ let encrypt_and_sign_message #a sender receiver payload pk_receiver sk_sender en
 // to create and parse confidential and authenticated messages.
 [@@ "opaque_to_smt"]
 val send_confidential_authenticated:
+  {|comm_layer_event_core_tag|} ->
   #a:Type -> {| parseable_serializeable bytes a |} ->
   communication_keys_sess_ids ->
   principal -> principal -> a ->
   traceful (option timestamp)
-let send_confidential_authenticated #a comm_keys_ids sender receiver payload =
+let send_confidential_authenticated #event_tag #a comm_keys_ids sender receiver payload =
   let*? pk_receiver = get_public_key sender comm_keys_ids.pki (LongTermPkeKey comm_layer_pkenc_tag) receiver in
   let*? sk_sender = get_private_key sender comm_keys_ids.private_keys (LongTermSigKey comm_layer_sign_tag) in
   let* enc_nonce = mk_rand PkeNonce (long_term_key_label sender) 32 in
@@ -229,11 +235,12 @@ let verify_and_decrypt_message #a #ps receiver sk_receiver vk_sender msg_encrypt
 
 [@@ "opaque_to_smt"]
 val receive_confidential_authenticated:
+  {|comm_layer_event_core_tag|} ->
   #a:Type -> {| parseable_serializeable bytes a |} ->
   communication_keys_sess_ids ->
   principal -> timestamp ->
   traceful (option (communication_message a))
-let receive_confidential_authenticated #a comm_keys_ids receiver msg_id =
+let receive_confidential_authenticated #event_tag #a comm_keys_ids receiver msg_id =
   let*? msg_encrypted_signed = recv_msg msg_id in
   let*? sk_receiver = get_private_key receiver comm_keys_ids.private_keys (LongTermPkeKey comm_layer_pkenc_tag) in
   let*? sender = return (get_sender msg_encrypted_signed) in
